A few more proofs and a start to a helpful lemma.

graph_inst.v
@@ -40,11 +40,16 @@ Module Bleh : Graphs PositiveOrderedTypeBits.
       | Node x s g' => mset.add x (vertices g')
     end.
 
+  Fixpoint edges' g : node_setPair :=
+    match g with
+      | Empty => msetPair.empty
+      | Node x s g' =>  msetPair.union (mset.fold (fun x' s'=> msetPair.add (x,x') s') s msetPair.empty) (edges' g')
+    end.
+
   Fixpoint edges g : node_setPair :=
     match g with 
       | Empty => msetPair.empty
-      | Node x s g' => mset.fold
-                        (fun x' s' => msetPair.add (x,x') s')
+      | Node x s g' => mset.fold (fun x' s' => msetPair.add (x,x') s')
                         s (edges g')
     end.
 
@@ -56,13 +61,13 @@ Module Bleh : Graphs PositiveOrderedTypeBits.
     fun g (x : node*node)  =>
       let (x1, x2) := x in
       if (mset.mem x1 (vertices g) && mset.mem x2 (vertices g))
-      then Node x1 ([x2]) g
+      then Node x1 (mset.add x2 mset.empty) g
       else g.
   Fixpoint remove_vertex (g : graph) (n : node) :=
   match g with
   |Empty => Empty
   |Node n' adj g' => if Pos.eqb n' n then remove_vertex g' n
-      else  Node n' adj g' (* this works because of the way edges are added.*)
+      else  Node n' adj (remove_vertex g' n)
   end.
 
 Fixpoint remove_edge (g : graph) (e : (node * node) ) :=
@@ -70,7 +75,7 @@ Fixpoint remove_edge (g : graph) (e : (node * node) ) :=
   let y := (snd e) in
   match g with
   |Empty => Empty
-  |Node n adj g' => if Pos.eqb n x && (Nat.eqb (mset.cardinal adj) 1)(*probably don't need this*) && (mset.mem y adj)  then remove_edge g' e
+  |Node n adj g' => if Pos.eqb n x  then Node n (mset.remove y adj) (remove_edge g' e)
                    else Node n adj (remove_edge g' e)
   end.
 
@@ -93,6 +98,83 @@ Fixpoint neighborhood (g : graph) (x : node) : node_set:=
   Proof. reflexivity. Qed.
   Lemma empty_edges : edges empty = msetPair.empty.
   Proof. reflexivity. Qed.
+
+  Lemma node_edges_weaken : forall (g : t) (n x y : node) n0  (e :=(x, y) : node * node),
+      msetPair.In (x,y) (edges (Node n n0 g)) ->
+      x = n /\ mset.In y n0 \/ msetPair.In e (edges g).
+    Proof.
+      intros.
+      apply mset_prop.set_induction.
+      intros.
+      destruct e.
+      left.
+      unfold edges in H.
+      induction g.
+    Admitted.
+
+  Lemma node_pres_verts : forall (n : node) (e : node_set) (g : t),
+      mset.Equal (vertices (Node n e g)) (mset.union (mset.add n mset.empty) (vertices g)).
+  Proof.
+    intros.
+    induction g.
+    simpl.
+    intros.
+    rewrite mset_prop.empty_union_2.
+    reflexivity. auto.
+    simpl.
+    intros.
+    rewrite mset_prop.add_union_singleton.
+    apply  mset_prop.union_equal_1.
+    apply mset_prop.singleton_equal_add.
+  Qed.
+
+  Definition pairset_of_nodes (n : node) (e : node_set) :=
+    mset.fold (fun (x : node) l => msetPair.add (n, x) l) e msetPair.empty.
+
+  Lemma node_pres_edges  : forall (n : node) (e : node_set)  (g : graph),
+      msetPair.Equal (edges (Node n e g))
+  (msetPair.union (pairset_of_nodes n e) (edges g)).
+  Proof.
+    intros.
+    simpl.
+    generalize (edges g).
+    intro n0.
+    set (P := fun e => ( msetPair.Equal
+     (mset.fold
+        (fun (x' : mset.elt) (s' : msetPair.t) =>
+         msetPair.add (n, x') s') e n0)
+     (msetPair.union (pairset_of_nodes n e) n0))).
+    change (P e).
+    apply mset_prop.set_induction.
+    intros.
+    unfold P.
+
+    rewrite mset_prop.fold_1b.
+    unfold pairset_of_nodes.
+    rewrite mset_prop.fold_1b.
+    rewrite msetPair_prop.empty_union_1.
+    reflexivity;
+    auto.
+    auto.
+    auto.
+    auto.
+    intros.
+    unfold P.
+    unfold pairset_of_nodes.
+    apply mset_prop.Add_Equal in H1.
+    rewrite mset_prop.fold_2.
+    Admitted.
+
+
+   Open Scope positive_scope.
+   Example ex1 : graph :=
+  Node 1 ([2,  3])
+       (Node 2 ([3])
+             (Node 3 [] Empty)).
+   
+   Compute (msetPair.elements (edges ex1)).
+   Compute (msetPair.elements (edges' ex1)).
+
   Lemma add_vertices :
     forall (x : node) (g : t), mset.In x (vertices (add_vertex g x)).
   Proof.
@@ -101,21 +183,6 @@ Fixpoint neighborhood (g : graph) (x : node) : node_set:=
     left; reflexivity.
   Qed.
 
-  Lemma add_edges_helper :
-    forall n n0 g,
-       msetPair.In (n, n0) (edges (Node n ([n0]) g)).
-    Proof.
-      intros.
-      induction g.
-      constructor; auto.
-      simpl. rewrite mset.fold_spec.
-      simpl. apply msetPair.add_spec.
-      auto.
-    Qed.
-
-    (* Lemma notin_vert_eq : *)
-    (*   forall ( *)
-   
   Lemma add_edges :
     forall (e : node * node) (g : t),
       mset.In (fst e) (vertices g) ->
@@ -125,33 +192,83 @@ Fixpoint neighborhood (g : graph) (x : node) : node_set:=
     intros. destruct e.
     induction g; simpl.
     inversion H.
-    apply mset.mem_spec in H; apply mset.mem_spec in H0.
-    case_eq (mset.mem n (mset.add n1 (vertices g)));
-      case_eq (mset.mem n0 (mset.add n1 (vertices g))).
-    simpl (_ && _); cbv iota.
+    simpl in H, H0.
+    apply mset.add_spec in H.
+    apply mset.add_spec in H0.    
+    destruct H, H0.
+    rewrite H, H0.
     {
-      intros H1 H2.
+      assert ( mset.mem n1 (mset.add n1 (vertices g)) = true).
+      rewrite mset.mem_spec.
+      apply mset_prop.Dec.F.add_iff.
+      auto.
+      rewrite H1.
+
+      simpl ( _ && _).
+      cbv iota.
       generalize (Node n1 n2 g).
-      intros. apply msetPair.add_spec.
+      intros.
+      
+      simpl.
+      apply msetPair.add_spec.
       auto.
     }
     {
-      intros H1 H2. 
+       assert ( mset.mem n (mset.add n1 (vertices g)) = true).
+      rewrite mset.mem_spec.
+      apply mset_prop.Dec.F.add_iff.
+      auto.
+      rewrite H1.
+      assert (mset.mem n0 (mset.add n1 (vertices g)) = true).
+      rewrite mset.mem_spec.
+      apply mset_prop.Dec.F.add_iff.
+      auto.
+      rewrite H2.
       simpl (_ && _); cbv iota.
-      admit.
+      generalize (Node n1 n2 g).
+      intro g0.
+      simpl.
+      apply msetPair.add_spec.
+      auto.
     }
     {
-      intros.
+      assert ( mset.mem n (mset.add n1 (vertices g)) = true).
+      rewrite mset.mem_spec.
+      apply mset_prop.Dec.F.add_iff.
+      auto.
+      rewrite H1.
+      assert (mset.mem n0 (mset.add n1 (vertices g)) = true).
+      rewrite mset.mem_spec.
+      apply mset_prop.Dec.F.add_iff.
+      auto.
+      rewrite H2.
       simpl ( _ && _); cbv iota.
-      apply msetPair.mem_spec.
-      admit.
+      generalize (Node n1 n2 g).
+      intro g0.
+      simpl.
+      apply msetPair.add_spec.
+      auto.
     }
     {
-      intros H1 H2.
-      simpl (_ && _); cbv iota.
-      admit.
-   }
-Admitted.
+      
+      assert ( mset.mem n (mset.add n1 (vertices g)) = true).
+      rewrite mset.mem_spec.
+      apply mset_prop.Dec.F.add_iff.
+      auto.
+      rewrite H1.
+      assert (mset.mem n0 (mset.add n1 (vertices g)) = true).
+      rewrite mset.mem_spec.
+      apply mset_prop.Dec.F.add_iff.
+      auto.
+      rewrite H2.
+      simpl ( _ && _); cbv iota.
+       generalize (Node n1 n2 g).
+      intro g0.
+      simpl.
+      apply msetPair.add_spec.
+      auto.
+    }
+  Qed.
 
     Lemma add_vertices_other :
       forall (x y : node) (g : t),
@@ -181,33 +298,22 @@ Admitted.
        auto.
     Qed.
 
-
-    Lemma in_add_edge_in_add :
-      forall e1 e2 g, msetPair.In e2 (edges (add_edge g e1)) ->msetPair.In e2 (msetPair.add e1 (edges (g))).
-      Proof.
-        intros.
-        induction g.
-        simpl. simpl in H.
-        Admitted.
-      
-
-
     Lemma add_edges_other :
       forall (e1 e2 : node * node) (g : t),
         e1 <> e2 -> msetPair.In e2 (edges g) <-> msetPair.In e2 (edges (add_edge g e1)).
     Proof.
       intros; split; induction g; auto.
       {
+       
        inversion 1.
       }
       {
         intros. unfold add_edge. 
         simpl.  destruct e1.
-        
         case_eq (mset.mem n1 (mset.add n (vertices g)));
           case_eq ( mset.mem n2 (mset.add n (vertices g))).
        
-          intros H1 H2; simpl (_ && _); cbv iota.
+        intros H1 H2; simpl (_ && _); cbv iota.
           apply msetPair.add_spec;
           auto.
           auto.
@@ -215,19 +321,16 @@ Admitted.
       }
       {
         intros.
-        unfold add_edge in H0.
-        simpl (_ && _) in H0. cbv iota in H0.
-        simpl (let (_, _) := e1 in Empty) in H0.
-        admit.
+        destruct e1.
+        auto.
       }
       {
         intros.
         apply msetPair_prop.Dec.F.add_3 with (x := e1).
-        auto. apply in_add_edge_in_add.
-        auto.
-      }
+        auto. rewrite msetPair.add_spec.
+        right.
     Admitted.
-       
+
     Lemma add_vertices_pres_edges :
       forall (x : node) (g : t), msetPair.Equal (edges (add_vertex g x)) (edges g).
     Proof.
@@ -242,7 +345,7 @@ Admitted.
       intros.
       unfold add_edge. destruct x.
       case_eq (mset.mem n (vertices g));
-        case_eq ( mset.mem n0 (vertices g)).
+      case_eq ( mset.mem n0 (vertices g)).
       {
         intros H1 H2; simpl. (*(_ && _); cbv iota.*)
         apply mset.mem_spec in H2.
@@ -264,21 +367,31 @@ Admitted.
     Proof.
       intros.
       induction g.
-      simpl. unfold not. intros. apply mset.mem_spec in H.
-      inversion H.
-      unfold not.
-      intros. apply mset.mem_spec in H. 
-      apply IHg.
-      apply mset.mem_spec in H.
+      simpl.
+      inversion 1.
+      unfold not in *.
+      intros.
       simpl in H.
+      destruct ((n =? x)%positive) in H.
+      apply IHg.
+      auto.
+      apply IHg.
+      apply node_pres_verts in H.
+      apply mset.union_spec in H.
+      destruct H eqn:H1.
+      Focus 2.
+      auto.
       Admitted.
-
+    
     Lemma remove_edges :
       forall (e : node * node) (g : t), ~ msetPair.In e (edges (remove_edge g e)).
     Proof.
       intros.
       unfold not. intros. induction g.
       inversion H.
+      simpl in H.
+      apply IHg.
+      destruct e.
       Admitted.
 
 
@@ -289,15 +402,25 @@ Admitted.
       intros. unfold not. intros.
       induction g.
       inversion H.
+      simpl in H.
+      auto.
     Admitted.
-    
+
+
+
     Lemma remove_vertices_edges_r :
         forall (x1 : node) (g : t) (x2 : node),
           ~ msetPair.In (x2, x1) (edges (remove_vertex g x1)).
     Proof.
+      unfold not.
       intros.
+      induction g.
+      inversion H.
+      apply IHg; auto.
+      simpl in H.
+      
     Admitted.
-    
+        
     Lemma remove_vertices_other :
         forall (x y : node) (g : t),
           x <> y ->  mset.In y (vertices g) <-> mset.In y (vertices (remove_vertex g x)).
@@ -315,13 +438,41 @@ Admitted.
       auto.
       auto.
       {
+        rewrite node_pres_verts in H0.
+        rewrite mset.union_spec in H0.
+        destruct H0.
+        rewrite <- mset_prop.singleton_equal_add in H0.
+        apply mset_prop.Dec.F.singleton_1 in H0.
+        Focus 2.
+        apply IHg.
+        apply H0.
         admit.
       }
-      
-      admit.
+      intros.
+      induction g.
+      inversion H0.
+      rewrite node_pres_verts.
+      apply mset.union_spec.
+      right.
     Admitted.
     
-    Lemma remove_edges_other :
+
+    Lemma in_edge_node_or_graph :
+      forall (g : t) n n0(e : node * node) ,
+        msetPair.In e (edges (Node n n0 g)) ->
+          (msetPair.In e (pairset_of_nodes n n0) \/ msetPair.In e (edges g)).
+    Proof.
+      intros.
+      generalize dependent g.
+      generalize dependent n.
+      generalize dependent n0.
+      induction g.
+      auto.
+      intros.
+      Admitted.
+      
+
+Lemma remove_edges_other :
       forall (e1 e2 : node * node) (g : t),
         e1 <> e2 -> msetPair.In e2 (edges g) <-> msetPair.In e2 (edges (remove_edge g e1)).
     Proof.
@@ -333,15 +484,13 @@ Admitted.
       {
         intro H1.
         simpl.
-        
-admit.
+        admit.
       }
       {
         auto.
       }
-
-
-
+      intros.
+      Admitted.
 
 
       Lemma is_vertex_vertices :
@@ -366,20 +515,45 @@ admit.
         intros; split. intros.  apply msetPair.mem_spec.
         induction g.
         inversion H.
-        destruct H.
-        subst.
-        simpl in H.
-Admitted.        
+        admit.
+        intros.
+        induction g.
+        inversion H.
+        simpl.
+      Admitted.        
 
-
-
-
-        
-
-      Parameter edges_proper_l :
+      Lemma edges_proper_l :
         forall (e : node * node) (g : t), msetPair.In e (edges g) -> mset.In (fst e) (vertices g).
-      Parameter edges_proper_r :
+      Proof.
+        intros.
+        induction g.
+        inversion H.
+        destruct e.
+        apply node_edges_weaken in H.
+        destruct H.
+        simpl.
+        apply mset.add_spec. 
+        destruct H.
+        auto.
+        apply IHg in H.
+        simpl.
+        apply mset.add_spec.
+        auto.
+Qed.
+      Lemma edges_proper_r :
         forall (e : node * node ) (g : t), msetPair.In e (edges g) -> mset.In (snd e) (vertices g).
+      Proof.
+        intros.
+        induction g.
+        inversion H.
+        simpl.
+        destruct e.
+        apply  node_edges_weaken in H.
+        destruct H.
+        simpl; apply mset.add_spec.
+        Admitted.
+
+
 End Bleh.
 Print Graphs.
 
